wip

clightplus/compiler_proof/ClightPlus2ClightSepComp.v
@@ -81,22 +81,41 @@ Section PROOFSINGLE.
   Arguments sloop_iter_body_two /.
   Arguments ktree_of_cont_itree /.
 
-  (* TODO: does semantics2 refine semantics2? *)
+  Definition inj sk ge b := Some (map_blk sk ge b, 0%Z).
+
+  Lemma mem2to3 sk_mem md clight_prog m tm tm' l:
+    match_mem (Sk.canon (Sk.add sk_mem (Mod.sk md))) (globalenv clight_prog) m tm ->
+    Genv.capture_init_mem tm l tm' -> 
+    Memory.Mem.mem_inj (inj (Sk.canon (Sk.add sk_mem (Mod.sk md))) (globalenv clight_prog)) m tm'.
+  Proof.
+    i. inv H. inv H0. Search Memory.Mem.capture_list.
+    Print Memdata.memval_inject.
+    Print Values.Val.inject.
+    Print Memory.Mem.flat_inj.
+    econs.
+    - i. unfold inj in *. clarify. replace (ofs + 0)%Z with ofs by nia.
+      unfold Memory.Mem.perm. rewrite MEM_PERM.
+    
+
   (* The thm is targeting closed program *)
   Theorem single_compile_behavior_improves
-          gvmap clight_prog md sk_mem mn left_st right_st
+          gvmap clight_prog md sk_mem mn left_st init_right_st right_st
           (COMP: compile clight_prog mn = Errors.OK md)
           (MEMSKEL: mem_skel clight_prog = Errors.OK sk_mem)
           (SINIT: left_st = clightp_initial_state sk_mem md)
-          (TINIT: Clight.initial_state clight_prog right_st)
+          (TINIT: Clight.initial_state clight_prog init_right_st)
+          (TCAP: glob_capture clight_prog init_right_st right_st)
         :
-          <<IMPROVES: @improves2 _ (semantics3 clight_prog) gvmap left_st right_st>>.
+          <<IMPROVES: @improves2 _ (semantics2 clight_prog) gvmap left_st right_st>>.
   Proof.
     eapply adequacy; eauto.
-    { apply Clight_wf_semantics. }
-    red. ss; clarify. unfold clightp_initial_state. ss; clarify. inv TINIT.
+    { 
+      (* apply Clight_wf_semantics.  *)
+      admit.
+      }
+    red. ss; clarify. unfold clightp_initial_state. ss; clarify. inv TINIT. inv TCAP.
     unfold ModSemL.initial_itr. unfold ge in *. clear ge.
-    rename H into INIT_TMEM, H0 into TMAINN_TBLOCK, H1 into TBLOCK_TMAINF, H2 into TMAIN_TYPE, f into tmainf.
+    rename H into INIT_TMEM, H0 into TMAINN_TBLOCK, H1 into TBLOCK_TMAINF, H2 into TMAIN_TYPE, f into tmainf, CAPTURE into INIT_TMEM_CAP.
 
     (* remove not-wf-(mem+md) case *)
     unfold ModL.wf_bool. destruct ModL.wf_dec; ss; [|sim_triggerUB].
@@ -191,20 +210,6 @@ Section PROOFSINGLE.
       repeat (des_ifs; progress (sim_redE; grind)). }
   Qed.
 
-  Theorem backward_simulation_observation_improves:
-  forall L, forall obs gvmap, program_observes L obs -> fst obs = Some gvmap ->
-    exists tr_src, program_observes L (Some null_map, tr_src) /\ observation_improves (Some null_map, tr_src) obs.
-  Proof.
-    i. inv H; clarify.
-    - ss. clarify. exists beh. split.
-      + econs. et. {  }
-       { econs; et. }
-    2:{ exists (Goes_wrong []). split. { econs 2. et. }
-        unfold observation_improves. ss. split. { unfold behavior_improves. left. ss. econs. }
-        ss. }
-    Semantics_gen
-       exists (Partial_terminates []). split. { econs 2. } }
-
   Theorem single_compile_program_improves
           clight_prog md sk_mem mn
           (COMP: compile clight_prog mn = Errors.OK md)
@@ -213,12 +218,7 @@ Section PROOFSINGLE.
       <<IMPROVES: improves2_program (clightp_sem sk_mem md) (Clight.semantics2 clight_prog)>>.
   Proof.
     red. unfold improves2_program. i. inv BEH; et.
-    { hexploit single_compile_behavior_improves.
-      { et. } { et. } { reflexivity. } { et. }
-      instantiate (1:=null_map).
-      unfold improves2, clightp_initial_state. i.
-      Search state_behaves.
-      eapply H; et. }
+    { eapply single_compile_behavior_improves; et. }
     (* initiall wrong case, for us only when main is not found *)
     exists (Tr.ub). split; red; eauto.
     2:{ pfold. econs 4; eauto.
